extracted Specs.SeqExt.mem (& related) into separate Seq.Mem.*

src/Flutterbye.Seq.Mem.fsi
@@ -1,0 +1,69 @@
+(*--build-config
+   options:--admit_fsi FStar.Seq;
+   other-files:seq.fsi
+--*)
+
+// $legal:614:
+//
+// Copyright 2015 Michael Lowell Roberts
+//
+// Licensed under the Apache License, Version 2.0 (the "License");
+// you may not use this file except in compliance with the License.
+// You may obtain a copy of the License at
+//
+//     http://www.apache.org/licenses/LICENSE-2.0
+//
+// Unless required by applicable law or agreed to in writing, software
+// distributed under the License is distributed on an "AS IS" BASIS,
+// WITHOUT WARRANTIES OR CONDITIONS OF ANY KIND, either express or implied.
+// See the License for the specific language governing permissions and
+// limitations under the License.
+//
+// ,$
+
+module Flutterbye.Seq.Mem
+   open FStar.Seq
+
+   val mem: seq 'a -> 'a -> Tot bool
+
+   val lemma__basic:
+      s: seq 'a
+      -> a: 'a
+      -> Lemma
+         (requires (True))
+         (ensures
+            ((mem s a)
+               <==>
+                  (exists i.
+                     0 <= i
+                     && i < length s
+                     && index s i = a)))
+         [SMTPat (mem s a)]
+
+   val lemma__slice:
+      s0: seq 'a
+      -> a: 'a
+      -> s1: seq 'a
+      -> j: nat{j <= length s1}
+      -> i: nat{0 <= i && i <= j}
+      -> Lemma
+         (requires (mem s0 a))
+         (ensures (Eq s0 (slice s1 i j) ==> mem s1 a))
+         [SMTPat (mem (slice s1 i j) a)]
+
+   val lemma__index:
+      s:seq 'a{length s > 0}
+      -> i:nat{i < length s}
+      -> Lemma
+         (requires (True))
+         (ensures (mem s (index s i)))
+         [SMTPat (mem s (index s i))]
+
+   val lemma__append:
+      s0: seq 'a
+      -> s1: seq 'a
+      -> a: 'a
+      -> Lemma
+         (requires (True))
+         (ensures (mem s0 a || mem s1 a <==> mem (append s0 s1) a))
+         [SMTPat (mem (append s0 s1) a)]
