src/Flutterbye.Seq.Mem.fst
@@ -1,0 +1,69 @@
+(*--build-config
+   options:--admit_fsi FStar.Seq --admit_fsi Flutterbye.Seq.Find;
+   other-files:seq.fsi Flutterbye.Seq.Find.fsi Flutterbye.Seq.Mem.fsi
+--*)
+
+// $legal:614:
+//
+// Copyright 2015 Michael Lowell Roberts
+//
+// Licensed under the Apache License, Version 2.0 (the "License");
+// you may not use this file except in compliance with the License.
+// You may obtain a copy of the License at
+//
+//     http://www.apache.org/licenses/LICENSE-2.0
+//
+// Unless required by applicable law or agreed to in writing, software
+// distributed under the License is distributed on an "AS IS" BASIS,
+// WITHOUT WARRANTIES OR CONDITIONS OF ANY KIND, either express or implied.
+// See the License for the specific language governing permissions and
+// limitations under the License.
+//
+// ,$
+
+module Flutterbye.Seq.Mem
+   open FStar.Seq
+   open Flutterbye.Seq.Find
+
+   let mem s a =
+      is_Some (find s a)
+
+   let lemma__basic s a =
+      ()
+
+   let lemma__index s i =
+      Flutterbye.Seq.Find.lemma__basic s (index s i)
+
+   let lemma__slice s0 a s1 j i =
+      ()
+
+   val lemma__append__case1:
+      s0: seq 'a
+      -> s1: seq 'a
+      -> a: 'a
+      -> Lemma
+         (requires (True))
+         (ensures (mem s0 a ==> mem (append s0 s1) a))
+   let lemma__append__case1 s0 s1 a =
+      ()
+
+   val lemma__append__case2:
+      s0: seq 'a
+      -> s1: seq 'a
+      -> a: 'a
+      -> Lemma
+         (requires (True))
+         (ensures (mem s1 a ==> mem (append s0 s1) a))
+   let lemma__append__case2 s0 s1 a =
+      if mem s1 a then
+         let s' = append s0 s1 in
+         let i = length s0 in
+         let j = length s' in
+         let s1' = slice s' i j in
+         lemma__slice s1' a s' j i
+      else
+         ()
+
+   let lemma_mem__append s0 s1 a =
+      lemma__append__case1 s0 s1 a;
+      lemma__append__case2 s0 s1 a
